---
layout: post
title: Introduction to sum
header-includes:
    - \usepackage{amsmath}
tags: [concrete_mathematics,sum]
comments: true
---
Sums are the fundamental objects in concrete mathematics. This post gives you a glimpse of them and sets the base for your further study. It will introduce to you the multiple notations of sums, the basic ways to manipulate sums and the ways to tackle sums with multiple indices.
## Notations
The simplest way to express a sum is $$a_1+a_2+...+a_n$$. The `...` represents the pattern of the sum. For example, the sum of all natural numbers from $$1$$ to $$n$$ is $$1+2+...+n$$.  
In some cases, the above pattern is rather elaborated, so mathematicians have thought of multiple ways to make summation notation more concise. The first of these alternative notations is the `sigma notataion` $$\sum$$. Using this notation, the sum of all natural numbers from $$1$$ to $$n$$ can be written as $$\sum_{i=1}^n a_i$$. We can generalize this form by specifying the predicate that the summands (aka $$a_i$$) must satisfy. Formally, this notation has the form $$\sum_{P_k} a_k$$, where $$P_k$$ is the predicate. For example, the equivalent of $$\sum_{k=0}^{49} (2k+1)$$ in the generalized form is $$ \sum_{\substack{1 \le k \le 100 \\ k \ \text{odd}}} k $$. This is the sum of all odd numbers from 1 to 99.  
Instead of writing the predicate under the $$\sum$$ notation, we can employ the Iverson's notation. The convention is to enclose the predicate by square brackets.  
$$
[P] = \begin{cases}
1 &\text{P is true} \\
0 &\text{P is false}
\end{cases}
$$  


For example, we can use Iverson's notation to express the predicate $$k \ \text{odd}$$ as follow.
$$  
[k \ \text{odd}] = \begin{cases}
1 &\text{P is odd} \\
0 &\text{P is even}
\end{cases}
$$  

With this new notation, the above sum of odd numbers from $$1$$ to $$99$$ can be expressed concisely with the Iverson's notation.  
$$
\begin{align}
\sum_k k[k \ \text{odd}, 1 \le k \le 100]
\end{align}
$$  

## Manipulation of sums
The first question to ask when we are given a sum is *What is the closed form of this sum?*. One strategy to answer this question is to convert the sum to another form that is easier to solve or closer to the closed form. To make that transformation feasible, we need to know some basic rules.  
Let $$K$$ be a set of finite integer numbers, sums over the elements of $$K$$ satisfy three rules.  
* **Distributive law**  
$$  
\begin{align}
\sum_{k \in K} ca_k = c\sum_{k \in K} a_k
\end{align}
$$  
* **Associative law**  
$$
\begin{align}
\sum_{k \in K} (a_k+b_k) = \sum_{k \in K} a_k + \sum_{k \in K} b_k
\end{align}
$$  
* **Commutative law**  
$$
\begin{align}
\sum_{k \in K} a_k = \sum_{p(k) \in K} a_{p(k)}
\end{align}
$$  

In the last rule, $$P{(k)}$$ is a permutation of $$K$$.  
Let's use these rules to find the closed form of the sum $$S_n=\sum_{0 \le k \le n} (a+bk)$$. When $$a=0$$ and $$b=1$$, this sum reduces to the sum of natural numbers which's closed form was found out by *Carl Friedrich Gauss* when he was 7.  
By using commutative law, we can replace $$k$$ with $$n-k$$. The given sum becomes $$S_n=\sum_{0 \le n-k \le n} (a+b(n-k))$$. Adding these two forms of the given sum, we have  

$$  
\begin{align}
2S_n&=\sum_{0 \le k \le n} (a+bk+a+b(n-k)) \\
&= \sum_{0 \le k \le n} (2a+bn) \\ 
&= (2a+bn)\sum_{0 \le k \le n} 1 \\
&= (2a+bn)(n+1)  
\end{align}
$$  

This gives us the closed form of the sum 
$$
S_n = \frac{(2a+bn)(n+1)}{2}  
$$  
The result can be interpreted as the average of the first term $$a$$ and the last term $$a+bn$$ times the number of term $$n+1$$.  
Besides associative, commutative, distributive laws of sum, Iverson's notation can help a lot in our quest to find transformation. For instance, the notation helps us make sense of the following identity  
$$
\begin{align}
\sum_{k \in K} a_k + \sum_{k \in K'} a_k = \sum_{k \in K \cup K'} a_k + \sum_{k \in K \cap K'} a_k
\end{align}
$$  

Rewriting the LHS using Iversion's notation and using the property $$[k \in K] + [k \in K'] = [k \in K \cup K'] + [k \in K \cap K']$$ gives us

$$
\begin{align}
LHS &= \sum_{k \in K} a_k + \sum_{k \in K'} a_k \\
&= \sum_k a_k[k \in K] + \sum_k a_k[k \in K'] \\
&= \sum_k a_k([k \in K] + [k \in K']) \\
&= \sum_k a_k([k \in K \cup K'] + [k \in K \cap K']) \\
&= \sum_k a_k[K \in K \cup K'] + \sum_k a_k[K \in K \cap K'] \\
&= \sum_{k \in K \cup K'} a_k + \sum_{k \in K \cap K'} a_k \\
&= RHS
\end{align}
$$  
Two common applications of this formula is to combine or split sum.  
* **Combine sum**  
$$
\begin{align}
\sum_{k=1}^{m} a_k + \sum_{k=m}^{n} a_k = a_m + \sum_{k=1}^{n} a_k
\end{align}
$$  
* **Split sum**  
$$
\begin{align}
\sum_{k=0}^{n} a_k = a_0 + \sum_{k=1}^{n} a_k
\end{align}
$$  


The operation of splitting sum has another name that is `perturbation method`. This method involves writing the sum $$S_{n+1}$$ in two ways.  
$$
\begin{align}
S_{n+1} = S_n + a_{n+1} = a_0 + \sum_{1 \le k \le n+1} a_k
\end{align}
$$  
Using the commutative law as above, we have $$\sum_{1 \le k \le n+1} a_k = \sum_{1 \le k+1 \le n+1} a_{k+1} = \sum_{0 \le k \le n} a_{k+1}$$.  

Thus 
$$
\begin{align}
S_{n+1} = S_n + a_{n+1} = a_0 + \sum_{0 \le k \le n} a_{k+1} \ (1)
\end{align}
$$  

To see the application of $$(1)$$, let's consider the following sum  
$$  
\begin{align}
S_n = \sum_{0 \le k \le n} k2^k
\end{align}
$$  

Applying $$(1)$$ to this sum, we have  
$$  
\begin{align}
S_{n+1} = S_n + (n+1)2^{n+1} = \sum_{0 \le k \le n} (k+1)2^{k+1} \ (2)
\end{align}
$$  

Now, let's consider the sum on the RHS  
$$
\begin{align}
\sum_{0 \le k \le n} (k+1)2^{k+1} = 2S_n + \sum_{0 \le k \le n}2^{k+1}
\end{align}
$$  


The remaining sum is a geometric progression, so $$\sum_{0 \le k \le n}2^{k+1} = 2^{n+2}-2$$.  
Hence, simplifying $$(2)$$ gives us the closed form $$S_n = (n-1)2^{n+1}+2$$.  

## Multiple sums
We use the same notations to represent sums that have more than one index. For example, consider this sum $$S_n=\sum_{1 \le i, j \le n} a_ib_j$$. The terms of this sum are governed by two indices $$i$$ and $$j$$. This sum can be rewritten by using the Iverson's notation $$S_n=\sum_{i,j}a_ib_j[1 \le i, j \le n]$$.  

Combining this and the fact that  
$$[1 \le i, j \le n] = [1 \le i \le n][1 \le j \le n]$$  
we can further transform this sum   
$$
\begin{align}
S_n &=\sum_{i,j}a_ib_j[1 \le i \le n][1 \le j \le n] \\ &= \sum_i a_i[1 \le i \le n] \sum_j b_j[1 \le j \le n] \\ & = \sum_{1 \le i \le n} a_i \sum_{1 \le j \le n} b_j
\end{align}
$$.  


The most important thing to remember in this section is the rules to interchange sums. It is easy to interchange sums if they are separated.  
$$  
\begin{align}
\sum_{j \in J}\sum_{k \in K} a_{j,k} = \sum_{k \in K}\sum_{j \in J} a_{j,k}
\end{align}
$$  

Things become harder when there is a relationship between indices. In that case, we can resort to Iverson's notation to support the interchanging operations. The general rule for the sum that have two indices is  
$$
\begin{align}
\sum_{j \in J}\sum_{k \in K(j)} a_{j, k} = \sum_{k \in K'}\sum_{j \in J'(k)} a_{j, k}  
\end{align}
$$


$$J$$, $$K$$, $$J'$$, $$K'$$ must satisfy the following relation  
$$
[j \in J][k \in K(j)] = [k \in K'][j \in J'(k)]  
$$  


One of the most common example of this rule is  
$$  
[1 \le j \le n][j \le k \le n] = [1 \le j \le k \le n] = [1 \le k \le n][1 \le j \le k]
$$  


Hence,  
$$
\begin{align}
\sum_{1 \le j \le n}\sum_{j \le k \le n} a_{j, k} = \sum_{1 \le j \le k \le n} a_{j, k} = \sum_{1 \le k \le n} \sum_{1 \le j \le k} a_{j, k}
\end{align}
$$  


Being equipped by the new tool, we will tackle a sum that is more complicated than the ones we saw before.  
$$
\begin{align}
S_n = \sum_{1 \le i < j \le n} (a_j-a_i)*(b_j-b_i)
\end{align}
$$  


Swapping $$i$$ and $$j$$ gives us and equivalent sum  
$$
\begin{align}
S_n &= \sum_{1 \le i < j \le n} (a_j-a_i)(b_j-b_i) \\ 
&= \sum_{1 \le j < i \le n} (a_i-a_j)(b_i-b_j) \\ 
&= \sum_{1 \le j < i \le n} (a_j-a_i)(b_j-b_i)
\end{align}
$$  


It's the time to apply our new formula. First, we have
$$
[1 \le i < j \le n] + [1 \le j < i \le n]  = [1 \le i, j \le n] - [1 \le i = j \le n]
$$  


Thus  
$$
\begin{align}
2S_n &= \sum_{1 \le i < j \le n} (a_j-a_i)(b_j-b_i) + \sum_{1 \le j < i \le n} (a_j-a_i)(b_j-b_i) \\ 
&= \sum_{1 \le i, j \le n}(a_j-a_i)(b_j-b_i)
\end{align}
$$  


Now, the RHS is easier to evaluate,  
$$
\begin{align}
 \sum_{1 \le i, j \le n}(a_j-a_i)(b_j-b_i) = 2n\sum_{1 \le i \le n} a_ib_i - 2(\sum_{1 \le i \le n}a_i)(\sum_{1 \le i \le n}b_i)
\end{align}
$$  

Hence we have the final identity  
$$
\begin{align}
(\sum_{1 \le i \le n}a_i)(\sum_{1 \le i \le n}b_i) = n\sum_{1 \le i \le n}a_ib_i - \sum_{1 \le i < j \le n}(a_j-a_i)(b_j-b_i)
\end{align}
$$  


From this identity, we can derive the `Chebysev's monotonic inequalities`.  
$$
\begin{align}
\text{if} \ a_1 \le a_2 \le ... \le a_n \ \text{and} \ b_1 \le b_2 \le ... \le b_n \ \text{then} \ (\sum_{i=1}^n a_i)(\sum_{i=1}^n a_j) \le n\sum_{i=1}^n a_ib_i 
\end{align}
$$  

and  
$$
\begin{align}
\text{if} \ a_1 \le a_2 \le ... \le a_n \ \text{and} \ b_1 \ge b_2 \ge ... \ge b_n \ \text{then} \ (\sum_{i=1}^n a_i)(\sum_{i=1}^n a_j) \ge n\sum_{i=1}^n a_ib_i 
\end{align}
$$  


There are still many things we need to study about sums and they are the subject of fundamental posts. For more information, you can read *Chapter 2* of the book `Concrete Mathematics` by Donald Knuth, which is the main source that this book is based on. In the next post, I will discuss about the general methods to find the closed form of a sum and go over examples. See you then.
